acl2/asl/static-env-replace.lisp
@@ -1,0 +1,606 @@
+;;****************************************************************************;;
+;;                                ASLRef                                      ;;
+;;****************************************************************************;;
+;;
+;; SPDX-FileCopyrightText: Copyright 2025 Arm Limited and/or its affiliates <open-source-office@arm.com>
+;; SPDX-License-Identifier: BSD-3-Clause
+;; 
+;;****************************************************************************;;
+;; Disclaimer:                                                                ;;
+;; This material covers both ASLv0 (viz, the existing ASL pseudocode language ;;
+;; which appears in the Arm Architecture Reference Manual) and ASLv1, a new,  ;;
+;; experimental, and as yet unreleased version of ASL.                        ;;
+;; This material is work in progress, more precisely at pre-Alpha quality as  ;;
+;; per Arm’s quality standards.                                               ;;
+;; In particular, this means that it would be premature to base any           ;;
+;; production tool development on this material.                              ;;
+;; However, any feedback, question, query and feature request would be most   ;;
+;; welcome; those can be sent to Arm’s Architecture Formal Team Lead          ;;
+;; Jade Alglave <jade.alglave@arm.com>, or by raising issues or PRs to the    ;;
+;; herdtools7 github repository.                                              ;;
+;;****************************************************************************;;
+
+(in-package "ASL")
+
+(include-book "interp")
+(include-book "std/util/defret-mutual-generate" :dir :System)
+(include-book "std/util/defconsts" :dir :system)
+(local (include-book "interp-theory"))
+
+
+
+(include-book "static-env-preserved")
+
+(local (std::add-default-post-define-hook :fix))
+
+(define global-replace-static ((static static_env_global-p)
+                               (global global-env-p))
+  :returns (new-global global-env-p)
+  (change-global-env global :static static)
+  ///
+  (defret global-env->storage-of-<fn>
+    (equal (global-env->storage new-global)
+           (global-env->storage global)))
+
+  (defret global-env->stack_size-of-<fn>
+    (equal (global-env->stack_size new-global)
+           (global-env->stack_size global)))
+
+  (defret global-env->static-of-<fn>
+    (equal (global-env->static new-global)
+           (static_env_global-fix static)))
+
+  (defret <fn>-of-<fn>
+    (equal (global-replace-static static1 new-global)
+           (global-replace-static static1 global)))
+
+  (defret <fn>-with-self
+    (implies (equal (static_env_global-fix static) (global-env->static global))
+             (equal (global-replace-static static global)
+                    (global-env-fix global)))))
+
+
+(define env-replace-static ((static static_env_global-p)
+                            (env env-p))
+  :returns (new-env env-p)
+  (change-env env :global (global-replace-static static (env->global env)))
+  ///
+  (defret env->global-of-<fn>
+    (equal (env->global new-env)
+           (global-replace-static static (env->global env))))
+
+  (defret env->local-of-<fn>
+    (equal (env->local new-env)
+           (env->local env)))
+
+  (defthm env-replace-static-of-env
+    (equal (env-replace-static static (env global local))
+           (env (global-replace-static static global) local)))
+
+  (defret <fn>-of-<fn>
+    (equal (env-replace-static static1 new-env)
+           (env-replace-static static1 env)))
+
+  (defret <fn>-with-self
+    (implies (equal (static_env_global-fix static) (global-env->static (env->global env)))
+             (equal (env-replace-static static env)
+                    (env-fix env)))))
+
+(local (defconst *asl-*staticro-xdoc*
+         '(:parents (asl-tracing)
+           :short "Modified version of @(see asl-interpreter-mutual-recursion) that passes
+the static env as a separate, read-only argument."
+           :long "")))
+
+
+(local
+ (defun replace-static-envs (x)
+   (if (atom x)
+       x
+     (case-match x
+       (('global-env->static ('env->global . &) . &) 'static-env)
+       (& (cons (replace-static-envs (car x))
+                (replace-static-envs (cdr x))))))))
+
+(local (include-book "interp-mods"))
+
+(defconsts *asl-interp-fns*
+  (acl2::strip-cadrs
+   (keep-define-forms-in-list
+    (find-form-by-car
+     'defines *asl-interpreter-mutual-recursion-command*))))
+
+(defconsts *eval-staticro-substitution*
+  (pair-suffixed (append *asl-interp-fns*
+                         '(asl-interpreter-mutual-recursion))
+                 '-*staticro))
+
+(defmacro bind-env-with-static (body)
+  `(b* ((env (mbe :logic (env-replace-static static-env env)
+                  :exec env)))
+     ,body))
+
+(with-output
+  :off (event)
+  (make-event
+   (b* ((form *asl-interpreter-mutual-recursion-command*)
+        ;; Strip out the events after the /// (theorem about resolved-p-of-resolve-ty)
+        (form (strip-post-/// form))
+        ;; Strip out xdoc
+        (form (strip-xdoc form))
+        ;; Add xdoc topic for mutual recursion
+        (form (add-mutrec-xdoc *asl-*staticro-xdoc* form))
+        ;; Add xdoc topic for each function
+        (form (add-define-xdoc
+               "Version of @(see <NAME>) with static env passed as a separate read-only argument;
+                see @(see asl-interpreter-mutual-recursion-*staticro) for overview."
+               form))
+        ;; Substitute function names with their -*t suffixed forms.
+        (form (sublis *eval-staticro-substitution* form))
+        ;; Replace all invocations of (global-env->static (env->global env)) with the variable static-env.
+        (form (replace-static-envs form))
+        ;; Add guard saying static-env equals the one in env.
+        (form (add-define-guard '(equal (global-env->static (env->global env)) static-env) form))
+        ;; Wrap each form with binding of env to one with static-env inserted
+        (form (wrap-define-bodies 'bind-env-with-static form))
+        ;; Add the tracespec formal to each define form.
+        (form (add-define-formals '(((static-env static_env_global-p) 'static-env)) form))
+        ;; Disable the functions and verify guards.
+        (form (insert-after-///
+               (list
+                '(make-event
+                  `(in-theory (disable . ,(fgetprop 'eval_expr-*t-fn 'acl2::recursivep nil (w state)))))
+                ;; (equals-original-thm '*t (w state))
+                ;; '(verify-guards eval_expr-*staticro-fn)
+                )
+               form)))
+     `(progn (defconst *asl-interpreter-mutual-recursion-*staticro-form* ',form)
+             ,form))))
+
+
+
+
+
+
+
+
+
+(defret <fn>-of-env-replace-static
+  (equal (let ((env (env-replace-static static env))) <call>)
+         (env-replace-static static new-env))
+  :hints(("Goal" :in-theory (enable <fn>)))
+  :fn env-assign-global)
+
+(defret <fn>-of-env-replace-static
+  (equal (let ((env (env-replace-static static env))) <call>)
+         (env-replace-static static new-env))
+  :hints(("Goal" :in-theory (enable <fn>)))
+  :fn env-assign-local)
+
+(defret <fn>-of-env-replace-static
+  (b* ((new-res (let ((env (env-replace-static static env))) <call>)))
+    (equal new-res
+           (env_result-case res
+             :lk_local (lk_local (env-replace-static static (lk_local->val res)))
+             :lk_global (lk_global (env-replace-static static (lk_global->val res)))
+             :otherwise res)))
+  :hints(("Goal" :in-theory (enable <fn>)))
+  :fn env-assign)
+
+(defret <fn>-of-env-replace-static
+  (equal (let ((env (env-replace-static static env))) <call>)
+         (env-replace-static static new-env))
+  :hints(("Goal" :in-theory (enable <fn>)))
+  :fn pop_scope)
+
+(defret <fn>-of-env-replace-static
+  (equal (let ((env (env-replace-static static env))) <call>)
+         (env-replace-static static new-env))
+  :hints(("Goal" :in-theory (enable <fn>)))
+  :fn push_scope)
+
+(defret <fn>-of-env-replace-static
+  (equal (let ((env (env-replace-static static env))) <call>)
+         (mv v_step (env-replace-static static new-env)))
+  :hints(("Goal" :in-theory (enable <fn>)))
+  :fn eval_for_step)
+
+
+
+(defret <fn>-global-env-replace-static
+  (equal (let ((env (env-replace-static static env))) <call>)
+         (env-replace-static static new-env))
+  :hints(("Goal" :in-theory (enable <fn>)))
+  :fn declare_local_identifier)
+
+(defret <fn>-global-env-replace-static
+  (equal (let ((env (env-replace-static static env))) <call>)
+         (env-replace-static static new-env))
+  :hints(("Goal" :in-theory (enable <fn>)))
+  :fn declare_local_identifiers)
+
+(defret <fn>-global-env-replace-static
+  (equal (let ((env (env-replace-static static env))) <call>)
+         (env-replace-static static new-env))
+  :hints(("Goal" :in-theory (enable <fn>)))
+  :fn remove_local_identifier)
+
+
+
+(defret <fn>-replace-static
+  (equal (let ((env (env-replace-static static env))) <call>)
+         (env-replace-static static new-env))
+  :hints(("Goal" :in-theory (enable <fn>)))
+  :fn env-push-stack)
+
+(defret <fn>-call-env-replace-static
+  (equal (let ((call-env (global-replace-static static call-env))) <call>)
+         (env-replace-static static new-env))
+  :hints(("Goal" :in-theory (enable <fn>)))
+  :fn env-pop-stack)
+
+(defret <fn>-prev-env-replace-static
+  (equal (let ((prev-env (env-replace-static static prev-env))) <call>)
+         new-env)
+  :hints(("Goal" :in-theory (enable <fn>)))
+  :fn env-pop-stack)
+
+
+
+
+(defconst *eval_result-replace-static-template*
+  '(define <evalresult-name>-replace-static ((static static_env_global-p)
+                                            (x <evalresult-name>-p))
+     :returns (new-x <evalresult-name>-p)
+     (eval_result-case x
+       :ev_normal
+       (:@ :no-result (eval_result-fix x))
+       (:@ (not :no-result) (ev_normal (<result-name>-replace-static static x.res)))
+       :ev_throwing (change-ev_throwing x :env (env-replace-static static x.env))
+       :otherwise (eval_result-fix x))
+     ///
+     (defret eval_result-kind-of-<fn>
+       (equal (eval_result-kind new-x)
+              (eval_result-kind x)))
+
+     (:@ (not :no-result)
+      (defret ev_normal->res-of-<fn>
+        (implies (eval_result-case x :ev_normal)
+                 (equal (ev_normal->res new-x)
+                        (<result-name>-replace-static static (ev_normal->res x))))))
+
+     ;; (:@ (not :no-result)
+     ;;  (defret ev_normal-of-<result-name>-replace-static
+     ;;    (equal (ev_normal (<result-name>-replace-static static res))
+     ;;           (<evalresult-name>-replace-static static (ev_normal res)))))
+     
+     (defret ev_throwing->env-of-<fn>
+       (implies (eval_result-case x :ev_throwing)
+                (equal (ev_throwing->env new-x)
+                       (env-replace-static static (ev_throwing->env x)))))
+
+     (defret ev_throwing->throwdata-of-<fn>
+       (implies (eval_result-case x :ev_throwing)
+                (equal (ev_throwing->throwdata new-x)
+                       (ev_throwing->throwdata x))))
+
+     (defret ev_throwing->backtrace-of-<fn>
+       (implies (eval_result-case x :ev_throwing)
+                (equal (ev_throwing->backtrace new-x)
+                       (ev_throwing->backtrace x))))
+
+     ;; (defret ev_error->desc-of-<fn>
+     ;;   (implies (eval_result-case x :ev_error)
+     ;;            (equal (ev_error->desc new-x)
+     ;;                   (ev_error->desc x))))
+
+     ;; (defret ev_error->data-of-<fn>
+     ;;   (implies (eval_result-case x :ev_error)
+     ;;            (equal (ev_error->data new-x)
+     ;;                   (ev_error->data x))))
+
+     ;; (defret ev_error->backtrace-of-<fn>
+     ;;   (implies (eval_result-case x :ev_error)
+     ;;            (equal (ev_error->backtrace new-x)
+     ;;                   (ev_error->backtrace x))))
+
+     
+     (defret <fn>-of-ev_error
+       (and (let ((x (ev_error data desc backtrace)))
+              (equal <call> x))
+            (implies (and (syntaxp (Quotep x))
+                          (eval_result-case x :ev_error))
+                     (equal new-x
+                            (eval_result-fix x)))))
+
+     (:@ (not :no-result)
+      (defret <fn>-when-not-normal
+        (implies (not (eval_result-case x :ev_normal))
+                 (equal new-x
+                        (eval_result-replace-static static x)))
+        :hints(("Goal" :in-theory (enable eval_result-replace-static)))))
+
+     (:@ (not :no-result)
+      (defret <fn>-when-error
+        (implies (eval_result-case x :ev_error)
+                 (equal new-x
+                        (eval_result-fix x)))))
+
+     (:@ :no-result
+      (defret <fn>-when-not-throwing
+        (implies (not (eval_result-case x :ev_throwing))
+                 (equal new-x
+                        (eval_result-fix x)))))))
+
+(defmacro def-eval_result-replace-static (evalresult-name
+                                          result-name)
+  (acl2::template-subst *eval_result-replace-static-template*
+                        :str-alist `(("<EVALRESULT-NAME>" . ,(symbol-name evalresult-name))
+                                     ("<RESULT-NAME>" . ,(symbol-name result-name)))
+                        :features (and (not result-name) '(:no-result))
+                        :pkg-sym 'asl-pkg))
+
+(def-eval_result-replace-static eval_result nil)
+
+(defthm eval_result-replace-static-of-ev_normal
+  (and (equal (eval_result-replace-static static (ev_normal res))
+              (ev_normal res))
+       (implies (and (syntaxp (Quotep x))
+                     (eval_result-case x :ev_normal))
+                (equal (eval_result-replace-static static x)
+                       (eval_result-fix x))))
+  :hints(("Goal" :in-theory (enable eval_result-replace-static))))
+
+
+
+
+(define expr_result-replace-static ((static static_env_global-p)
+                                    (x expr_result-p))
+  :returns (new-x expr_result-p)
+  (change-expr_result x :env (env-replace-static static (expr_result->env x)))
+  ///
+  (defret expr_result->val-of-<fn>
+    (equal (expr_result->val new-x)
+           (expr_result->val x)))
+
+  (defret expr_result->env-of-<fn>
+    (equal (expr_result->env new-x)
+           (env-replace-static static (expr_result->env x)))))
+
+(def-eval_result-replace-static expr_eval_result expr_result)
+
+(define exprlist_result-replace-static ((static static_env_global-p)
+                                    (x exprlist_result-p))
+  :returns (new-x exprlist_result-p)
+  (change-exprlist_result x :env (env-replace-static static (exprlist_result->env x)))
+  ///
+  (defret exprlist_result->val-of-<fn>
+    (equal (exprlist_result->val new-x)
+           (exprlist_result->val x)))
+
+  (defret exprlist_result->env-of-<fn>
+    (equal (exprlist_result->env new-x)
+           (env-replace-static static (exprlist_result->env x)))))
+
+(def-eval_result-replace-static exprlist_eval_result exprlist_result)
+
+(define func_result-replace-static ((static static_env_global-p)
+                                    (x func_result-p))
+  :returns (new-x func_result-p)
+  (change-func_result x :env (global-replace-static static (func_result->env x)))
+  ///
+  (defret func_result->vals-of-<fn>
+    (equal (func_result->vals new-x)
+           (func_result->vals x)))
+
+  (defret func_result->env-of-<fn>
+    (equal (func_result->env new-x)
+           (global-replace-static static (func_result->env x)))))
+
+(def-eval_result-replace-static func_eval_result func_result)
+
+
+(define control_flow_state-replace-static ((static static_env_global-p)
+                                           (x control_flow_state-p))
+  :returns (new-x control_flow_state-p)
+  (control_flow_state-case x
+    :returning (change-returning x :env (global-replace-static static x.env))
+    :continuing (change-continuing x :env (env-replace-static static x.env)))
+  ///
+  (defret control_flow_state-kind-of-<fn>
+    (equal (control_flow_state-kind new-x)
+           (control_flow_state-kind x)))
+
+  (defret returning->vals-of-<fn>
+    (equal (returning->vals new-x)
+           (returning->vals x))
+    :hints(("Goal" :in-theory (enable returning->vals-when-wrong-kind))))
+
+  (defret returning->env-of-<fn>
+    (implies (control_flow_state-case x :returning)
+             (equal (returning->env new-x)
+                    (global-replace-static static (returning->env x)))))
+
+  (defret continuing->env-of-<fn>
+    (implies (control_flow_state-case x :continuing)
+             (equal (continuing->env new-x)
+                    (env-replace-static static (continuing->env x))))))
+
+(def-eval_result-replace-static stmt_eval_result control_flow_state)
+
+(def-eval_result-replace-static env_eval_result env)
+
+
+(define intpair/env-replace-static ((static static_env_global-p)
+                                    (x intpair/env-p))
+  :returns (new-x intpair/env-p)
+  (change-intpair/env x :env (env-replace-static static (intpair/env->env x)))
+  ///
+  (defret intpair/env->pair-of-<fn>
+    (equal (intpair/env->pair new-x)
+           (intpair/env->pair x)))
+
+  (defret intpair/env->env-of-<fn>
+    (equal (intpair/env->env new-x)
+           (env-replace-static static (intpair/env->env x)))))
+
+(def-eval_result-replace-static slice_eval_result intpair/env)
+
+(define intpairlist/env-replace-static ((static static_env_global-p)
+                                        (x intpairlist/env-p))
+  :returns (new-x intpairlist/env-p)
+  (change-intpairlist/env x :env (env-replace-static static (intpairlist/env->env x)))
+  ///
+  (defret intpairlist/env->pairlist-of-<fn>
+    (equal (intpairlist/env->pairlist new-x)
+           (intpairlist/env->pairlist x)))
+
+  (defret intpairlist/env->env-of-<fn>
+    (equal (intpairlist/env->env new-x)
+           (env-replace-static static (intpairlist/env->env x)))))
+
+(def-eval_result-replace-static slices_eval_result intpairlist/env)
+
+(local (include-book "centaur/vl/util/default-hints" :dir :system))
+
+(local (defthm mv-nth-when-equal-cons
+         (implies (equal x (cons a b))
+                  (equal (mv-nth n x)
+                         (mv-nth n (cons a b))))))
+
+;; (local (defthm is_val_of_type_tuple-mv-nths
+;;          (let ((call (is_val_of_type_tuple env vals types)))
+;;            (equal (list (mv-nth 0 call) (mv-nth 1 call)) call))
+;;          :hints (("goal" :Expand ((is_val_of_type_tuple env vals types))))))
+
+
+(defret <fn>-of-stmt_eval_result-replace-static
+  (equal (let ((blkres (stmt_eval_result-replace-static static blkres))) <call>)
+         (stmt_eval_result-replace-static static res))
+  :hints(("Goal" :in-theory (enable <fn>)))
+  :fn rethrow_implicit)
+
+(defret <fn>-of-eval_result-replace-static
+  (implies (not (eval_result-case blkres :ev_normal))
+           (equal (let ((blkres (eval_result-replace-static static blkres))) <call>)
+                  (eval_result-replace-static static res)))
+  :hints(("Goal" :in-theory (enable <fn>)))
+  :fn rethrow_implicit)
+
+
+(defthm rethrow_implicit-when-not-throw
+  (implies (not (eval_result-case blkres :ev_throwing))
+           (equal (rethrow_implicit throw blkres backtrace)
+                  blkres))
+  :hints(("Goal" :in-theory (enable rethrow_implicit))))
+
+(defret env-find-global-of-env-replace-static
+  (equal (let ((env (env-replace-static static env))) <call>)
+         res)
+  :hints(("Goal" :in-theory (enable <fn>)))
+  :fn env-find-global)
+
+
+(defthm eval_limit-*staticro-mv-nths
+  (let ((res (eval_limit-*staticro env limit)))
+    (equal (list (mv-nth 0 res) (mv-nth 1 res)) res))
+  :hints (("goal" :expand ((eval_limit-*staticro env limit)))))
+
+(defthm stmt_eval_result-replace-static-when-ev_normal
+  (implies (eval_result-case x :ev_normal)
+           (equal (stmt_eval_result-replace-static static x)
+                  (ev_normal (control_flow_state-replace-static static (ev_normal->res x)))))
+  :hints(("Goal" :in-theory (enable stmt_eval_result-replace-static))))
+
+
+(defthm check_recurse_limit-of-global-replace-static
+  (equal (check_recurse_limit (env (global-replace-static static global) local) name limit)
+         (check_recurse_limit (env global local) name limit))
+  :hints(("Goal" :in-theory (enable check_recurse_limit get_stack_size))))
+
+
+
+
+(local
+ (defun staticro-equals-original-thms (names suffix wrld)
+   (if (atom names)
+       nil
+     (cons
+      (let* ((name (car names))
+             (name-mod (intern-in-package-of-symbol
+                        (concatenate 'string (symbol-name name) "-"
+                                     (symbol-name suffix))
+                        name))
+             (macro-args (macro-args name wrld))
+             (nonkey-formals (take (- (len macro-args)
+                                      (len (member '&key macro-args)))
+                                   macro-args)))
+        `(defret ,(intern-in-package-of-symbol
+                   (concatenate 'string "<FN>" "-EQUALS-ORIGINAL")
+                   'asl-pkg)
+           (equal (,name-mod . ,nonkey-formals)
+                  (let ((env (env-replace-static static-env env)))
+                    (,name . ,nonkey-formals)))
+           :hints ((let ((expand (acl2::just-expand-cp-parse-hints
+                                  '((:free (,@nonkey-formals clk orac) (,name-mod . ,nonkey-formals))
+                                    (:free (,@nonkey-formals clk orac) (,name . ,nonkey-formals)))
+                                  world)))
+                     `(:computed-hint-replacement
+                       ((acl2::expand-marked))
+                       :clause-processor (acl2::mark-expands-cp
+                                          clause
+                                          '(t ;; last-only
+                                            t ;; lambdas
+                                            ,expand))
+                       :do-not-induct t)))
+           :fn ,name-mod))
+      (staticro-equals-original-thms (cdr names) suffix wrld)))))
+
+(local
+ (defun staticro-equals-original-thm (suffix wrld)
+   `(encapsulate nil
+      (local (deflabel before-equals-original))
+      (std::defret-mutual
+        ,(intern-in-package-of-symbol (concatenate 'string (symbol-name suffix) "EQUALS-ORIGINAL") 'asl-pkg)
+        . ,(staticro-equals-original-thms *asl-interp-fns* suffix wrld))
+      (acl2::def-ruleset! asl-*staticro-equals-original-rules
+        (set-difference-theories (current-theory :here)
+                                 (current-theory 'before-equals-original))))))
+
+(with-output
+  :off (event)
+  :evisc (:gag-mode (evisc-tuple 3 4 nil nil))
+  (make-event
+   (staticro-equals-original-thm '*staticro (w state))))
+
+
+(local (in-theory (disable (tau-system)
+                           len assoc-equal append true-listp loghead hons-assoc-equal floor mod expt take
+                           acl2::repeat)))
+
+(local
+ (defthm eval_result-kind-of-rethrow_implicit
+   (equal (eval_result-kind (rethrow_implicit throw blkres backtrace))
+          (eval_result-kind blkres))
+   :hints(("Goal" :in-theory (enable rethrow_implicit)))))
+
+(local
+ (defthm ev_error->desc-of-rethrow_implicit
+   (implies (eval_result-case blkres :ev_error)
+            (equal (ev_error->desc (rethrow_implicit throw blkres backtrace))
+                   (ev_error->desc blkres)))
+   :hints(("Goal" :in-theory (enable rethrow_implicit)))))
+
+(with-output
+  :off (event)
+  (verify-guards eval_expr-*staticro-fn
+    :guard-debug t))
+             
+
+
+
+
+
+
+
+
